git/jrr6/lean-tables/Table/Proofs.lean
@@ -4,7 +4,6 @@ universe u u_η
 
 variable {η : Type u_η} [dec_η : DecidableEq η] {sch : @Schema η}
 
--- TODO: we shouldn't need to specify η here
 theorem emptyTable_spec1 : @schema η dec_η _ emptyTable = [] := rfl
 
 theorem emptyTable_spec2 : @nrows η dec_η _ emptyTable = 0 := rfl
@@ -19,7 +18,7 @@ theorem addRows_spec2 :
     nrows (addRows t rs) = nrows t + rs.length :=
 λ t rs => List.length_append (t.rows) rs
 
--- FIXME: deal with precondition 1
+-- TODO: deal with precondition 1
 -- We must enforce decidable equality of τ to state this theorem
 -- We omit the precondition because it is not required for this portion of the
 -- spec
@@ -32,9 +31,37 @@ theorem addColumn_spec1 :
   | nil => simp [List.map, List.append]
   | cons s ss ih =>
     simp only [List.map]
+    -- TODO: after updating to Lean 4 m4, these unfolds become necessary...
+    unfold HAppend.hAppend at ih
+    unfold instHAppend at ih
+    unfold Append.append at ih
+    unfold List.instAppendList at ih
+    simp only at ih
     rw [ih]
     simp [List.append]
-    -- FIXME: why does it want a Table ss here?!
+    -- FIXME: why does it want a Table ss?
+    exact Table.mk []
+
+-- ⟨cc.val,
+-- by cases cc with | mk val prop =>
+--    induction prop with
+--    | hd => apply Schema.HasName.hd
+--    | @tl r c' rs h ih =>
+--     apply Schema.HasName.tl
+--     simp only [schema, addColumn] at ih
+-- ⟩
+
+theorem addColumn_spec2 :
+  ∀ {τ : Type u}
+    (t : Table sch)
+    (c : η)
+    (vs : List τ)
+    (c' : η)
+    (h' : sch.HasName c'),
+    c ∈ header t →
+      (schema t).lookup ⟨c', h'⟩ =
+      (schema (addColumn t c vs)).lookup ⟨c', Schema.hasNameOfAppend h'⟩ :=
+λ t c vs c' h' h => Schema.lookup_eq_lookup_append _ _ _ _
 
 -- FIXME: how to show c is certifed?
 -- theorem addColumn_spec3 :
@@ -62,7 +89,6 @@ theorem addColumn_spec4 :
 --     sorry
 
 -- Spec 1 is enforced by the type system
--- FIXME: same issue as addColumn spec 1!
 theorem buildColumn_spec2 :
   ∀ {τ : Type u} (t : Table sch) (c : η) (f : Row sch → τ),
     header (buildColumn t c f) = List.append (header t) [c] :=
@@ -72,8 +98,26 @@ by intros τ t c f
   | nil => simp [List.map, List.append]
   | cons s ss ih =>
     simp only [List.map]
+    -- TODO: same issue with the ih
+    unfold HAppend.hAppend at ih
+    unfold instHAppend at ih
+    unfold Append.append at ih
+    unfold List.instAppendList at ih
+    simp only at ih
     rw [ih]
     simp [List.append]
+    -- FIXME: why does it want all of this?
+    exact Table.mk []
+    exact (λ x => f (Row.cons Cell.emp x))
+
+theorem buildColumn_spec5 :
+  ∀ {τ : Type u} (t : Table sch) (c : η) (f : Row sch → τ),
+    nrows (buildColumn t c f) = nrows t :=
+by intros τ t c f
+   simp only [nrows, buildColumn, addColumn]
+   rw [List.length_map, List.zip_length_eq_of_length_eq]
+   apply Eq.symm
+   apply List.length_map
 
 -- TODO: come back to buildColumn
 
@@ -131,6 +175,84 @@ theorem getColumn2_spec2 :
     List.length (getColumn2 t c h) = nrows t :=
 λ t c h => List.length_map _ _
 
+-- Precondition is enforced by subtype
+theorem selectRows1_spec1 :
+  ∀ (t : Table sch) (ns : List {n // n < nrows t}),
+    schema (selectRows1 t ns) = schema t :=
+λ t ns => rfl
+
+theorem selectRows1_spec2 :
+  ∀ (t : Table sch) (ns : List {n // n < nrows t}),
+    nrows (selectRows1 t ns) = ns.length :=
+λ t ns => List.length_map _ _
+
+-- Precondition is enforced by `h`
+theorem selectRows2_spec1 :
+  ∀ (t : Table sch) (bs : List Bool) (h : bs.length = nrows t),
+    schema (selectRows2 t bs h) = schema t :=
+λ t bs h => rfl
+
+theorem selectRows2_spec2 :
+  ∀ (t : Table sch) (bs : List Bool) (h : bs.length = nrows t),
+    nrows (selectRows2 t bs h) = (bs.removeAll [false]).length :=
+λ t bs h => List.sieve_removeAll _ _ h
+
+theorem selectColumns1_spec1 :
+  ∀ (t : Table sch) (bs : List Bool) (h : bs.length = ncols t),
+    List.Sublist (header (selectColumns1 t bs h)) (header t) :=
+λ t bs h => List.sublist_of_map_sublist _ _ Prod.fst $ List.sieve_sublist bs sch
+
+-- FIXME: there must be a better way
+theorem ncols_eq_header_length :
+  ∀ (t : Table sch), ncols t = (header t).length :=
+λ t => Eq.symm (List.length_map _ _)
+theorem selectColumns1_spec2 :
+  ∀ (t : Table sch) (bs : List Bool) (h : bs.length = ncols t) (i : Nat) (h' : i < ncols t),
+  (List.get (header t) ⟨i, (ncols_eq_header_length t).subst h'⟩) ∈ (header (selectColumns1 t bs h)) ↔
+   List.get bs ⟨i, Eq.subst h.symm h'⟩ = true := sorry
+
+theorem selectColumns1_spec3 :
+  ∀ (t : Table sch) (bs : List Bool) (h : bs.length = ncols t),
+    List.Sublist (schema (selectColumns1 t bs h)) (schema t) :=
+λ t bs h => List.sieve_sublist _ _
+
+theorem selectColumns1_spec4 :
+  ∀ (t : Table sch) (bs : List Bool) (h : bs.length = ncols t),
+    nrows (selectColumns1 t bs h) = nrows t :=
+λ t bs h => List.length_map _ _
+
+theorem selectColumns2_spec1 :
+  ∀ (t : Table sch) (ns : List {n // n < ncols t}),
+    ncols (selectColumns2 t ns) = ns.length :=
+λ t ns => List.length_map _ _
+
+-- TODO: sc2 specs 2 and 3
+
+theorem selectColumns2_spec4 :
+  ∀ (t : Table sch) (ns : List {n // n < ncols t}),
+    nrows (selectColumns2 t ns) = nrows t :=
+λ t ns => List.length_map _ _
+
+theorem selectColumns3_spec1 :
+  ∀ (t : Table sch) (cs : List (CertifiedName sch)),
+    header (selectColumns3 t cs) = cs.map Sigma.fst :=
+by intros t cs
+   simp only [header, selectColumns3, Schema.names]
+   induction cs with
+   | nil => simp only [Schema.pick, List.map]
+   | cons c cs ih =>
+     simp only [Schema.pick, List.map, List.cons.injEq]
+     apply And.intro
+     . simp only [Schema.lookup_fst_eq_nm, CertifiedName.val]
+     . exact ih
+
+-- TODO: sc3 spec 2
+
+theorem selectColumns3_spec3 :
+  ∀ (t : Table sch) (cs : List (CertifiedName sch)),
+    nrows (selectColumns3 t cs) = nrows t :=
+λ t cs => List.length_map _ _
+
 -- Spec 1 is enforced by types
 theorem head_spec2 : ∀ (t : Table sch) (z : {z : Int // z.abs < nrows t}),
   z.val ≥ 0 → nrows (head t z) = z.val :=
@@ -165,11 +287,3 @@ by intros t z h
 theorem dropColumn_spec3 : ∀ (t : Table sch) (c : CertifiedName sch),
   List.Sublist (schema (dropColumn t c)) (schema t) :=
 λ _ c => Schema.removeName_sublist sch c.val c.property
-
--- FIXME: there must be a better way
-theorem ncols_eq_header_length : ∀ (t : Table sch), ncols t = (header t).length :=
-λ t => Eq.symm (List.length_map _ _)
-theorem selectColumns1_spec2 :
-  ∀ (t : Table sch) (bs : List Bool) (h : bs.length = ncols t) (i : Nat) (h' : i < ncols t),
-  (List.get (header t) ⟨i, (ncols_eq_header_length t).subst h'⟩) ∈ (header (selectColumns t bs h)) ↔
-   List.get bs ⟨i, Eq.subst h.symm h'⟩ = true := sorry
